deps/poulet4/lib/P4cub/SmallStepTypeSoundness.v
@@ -247,17 +247,16 @@ Section ParserExprTheorems.
       π ϵ, e -->  e' -> ⟅ sts, errs, Γ ⟆ ⊢ e -> ⟅ sts, errs, Γ ⟆ ⊢ e'.
     Proof.
       intros e e' Hpi Ht; induction Hpi; inv Ht; repeat subst_term; eauto 3.
-      - econstructor; eauto 1; autorewrite with core in *;
+      (*- econstructor; eauto 1; autorewrite with core in *;
         unravel in *; intuition; inv_Forall_cons;
-        constructor; unravel in *; intuition; eauto 2.
-      - destruct (F.get v cases) as [? |] eqn:Hget; eauto.
+        constructor; unravel in *; intuition; eauto 2.*)
+      - destruct (F.find_value (fun _ => false) cases) as [? |] eqn:Hget; eauto.
         (* TODO: Need helper lemma for get. *)
-        clear d H6 H0 H.
+        clear d H5.
         generalize dependent e.
         induction cases as [| [e pe] cases ?];
         intros pst Hget; unravel in *;
-        try inv_Forall_cons; try discriminate.
-        destruct (equiv_dec v e) as [Hve | Hve]; unravel in *;
+          try inv_Forall_cons; try discriminate.
         inv_eq; intuition.
     Qed.
   End Preservation.
@@ -267,7 +266,7 @@ Section ParserExprTheorems.
     Hint Rewrite Forall_app : core.
     Hint Resolve value_exm : core.
 
-    Inductive select_expr : PS.e tags_t -> Prop :=
+    Inductive select_expr : PR.e tags_t -> Prop :=
       Select_select e d cases i :
         select_expr p{ select e { cases } default:=d @ i }p.
     (**[]*)
@@ -279,15 +278,6 @@ Section ParserExprTheorems.
     Proof.
       intros e Hs He; induction He using check_prsrexpr_ind; inv Hs.
       eapply expr_small_step_progress in H as [Hev | [e' He']]; eauto 3.
-      pose proof Forall_exists_prefix_only_or_all (value ∘ fst) cases
-        as [Hall | [[ee pe] [prf [suf [Heq [Hprf Hee]]]]]];
-      subst; autorewrite with core in *; eauto 3.
-      - intros [? ?]; unravel; auto 1.
-      - unravel in *; intuition; inv_Forall_cons;
-        intuition; unravel in *.
-        eapply expr_small_step_progress in H1 as [? | [ee' ?]];
-        eauto 1; try contradiction.
-        exists (PS.PSelect e def (prf ++ (ee', pe) :: suf) i); eauto 2.
     Qed.
   End Progress.
 End ParserExprTheorems.
